GCTR properties are subtle, but F* is baffling

src/crypto/aes/GCTR_i.fst
@@ -8,7 +8,9 @@ open GCTR_s
 
 let rec gctr_encrypt_recursive_length (icb:quad32) (plain:gctr_plain) 
 				      (alg:algorithm) (key:aes_key alg) (i:int) : 
-  Lemma(length (gctr_encrypt_recursive icb plain alg key i) == length plain) =
+  Lemma(length (gctr_encrypt_recursive icb plain alg key i) == length plain)
+  [SMTPat (length (gctr_encrypt_recursive icb plain alg key i))]
+  =
   match plain with 
   | [] -> ()
   | hd :: tl -> gctr_encrypt_recursive_length icb tl alg key (i + 1); 
@@ -33,6 +35,53 @@ let nth_in_bounds (l:list 'a) (i:int {0 <= i /\ i < length l}) =
   nth_in_bounds_is_some l i;
   Some?.v (nth l i)
 
+let nth_in_bounds_extension (l:list 'a) (i:int {0 < i /\ i < length l}) : Lemma
+  (requires length l > 0)
+  (ensures (nth_in_bounds l i) == (nth_in_bounds (Cons?.tl l) (i - 1)))
+  =
+  ()
+
+(*
+let rec gctr_indexed (icb:quad32) (plain:gctr_plain) 
+		     (alg:algorithm) (key:aes_key alg) (i:int) : Lemma
+  (requires True)
+  (ensures (let cipher = gctr_encrypt_recursive icb plain alg key i in
+	    length cipher == length plain /\
+	   (forall j . {:pattern nth_in_bounds cipher j} 0 <= j /\ j < length plain ==>
+	   nth_in_bounds cipher j == quad32_xor (nth_in_bounds plain j) (aes_encrypt alg key (inc32 icb (i + j)) ))))
+=
+  match plain with 
+  | [] -> ()
+  | hd :: tl ->
+      let cipher = gctr_encrypt_recursive icb plain alg key i in  
+      assert (length cipher == length plain);
+      let r_cipher = gctr_encrypt_recursive icb tl alg key (i+1) in     
+      assert( Cons?.tl cipher == r_cipher);
+      gctr_indexed icb tl alg key (i+1);
+      let foo (j:int{0 <= j /\ j < length plain}) : 
+	Lemma (nth_in_bounds cipher j == quad32_xor (nth_in_bounds plain j) (aes_encrypt alg key (inc32 icb (i + j)) ))
+	= 
+	if j = 0 then ()
+	else 
+	assert(j > 0);
+	assert(j < length plain);
+	assert(j < length cipher);
+	nth_in_bounds_extension cipher j;
+	assert(nth_in_bounds cipher j == nth_in_bounds r_cipher (j - 1));
+		assume(False);
+	assert(nth_in_bounds cipher (j-1) == quad32_xor (nth_in_bounds tl (j-1)) (aes_encrypt alg key (inc32 icb (i + j - 1)) ));
+	assume(False)
+      in
+      assume(False)
+(*      
+      assert (nth_in_bounds r_cipher (i-1) == quad32_xor (nth_in_bounds tl (i-1)) (aes_encrypt alg key (inc32 icb (i+1) )));
+      assert( Cons?.tl cipher == r_cipher);
+      //assert (nth_in_bounds r_cipher (i-1) == nth_in_bounds cipher i);
+      
+      assume(False)
+*)      
+
+
 let rec gctr_indexed (icb:quad32) (plain:gctr_plain) 
 		     (alg:algorithm) (key:aes_key alg) (i:int { 0 <= i /\ i < length plain }) : Lemma
   (requires True)
@@ -41,8 +90,50 @@ let rec gctr_indexed (icb:quad32) (plain:gctr_plain)
 	   (nth_in_bounds cipher i == quad32_xor (nth_in_bounds plain i) (aes_encrypt alg key (inc32 icb i) ))))
 =
   if i = 0 then ()
-  else (assume False)//; gctr_indexed icb (Cons?.tl plain) alg key (i - 1)
- 
+  else 
+    match plain with 
+    | [] -> ()
+    | hd :: tl -> 
+      let cipher = gctr_encrypt_recursive icb plain alg key 0 in  
+      let tl_cipher = gctr_encrypt_recursive icb tl alg key 1 in  
+      assert( Cons?.tl cipher == tl_cipher);
+      gctr_indexed icb plain alg key (i - 1);
+      assert (nth_in_bounds cipher (i-1) == quad32_xor (nth_in_bounds plain (i-1)) (aes_encrypt alg key (inc32 icb (i-1) )));
+      assume(False)
+
+
+      let r_cipher = gctr_encrypt_recursive icb tl alg key (i-1) in     
+      gctr_indexed icb tl alg key (i - 1);
+      assert (nth_in_bounds r_cipher (i-1) == quad32_xor (nth_in_bounds tl (i-1)) (aes_encrypt alg key (inc32 icb (i+1) )));
+      assert( Cons?.tl cipher == r_cipher);
+      //assert (nth_in_bounds r_cipher (i-1) == nth_in_bounds cipher i);
+      
+      assume(False)
+
+
+
+
+let rec gctr_indexed (icb:quad32) (plain:gctr_plain) 
+		     (alg:algorithm) (key:aes_key alg) (i:int { 0 <= i /\ i < length plain }) : Lemma
+  (requires True)
+  (ensures (let cipher = gctr_encrypt_recursive icb plain alg key i in
+	    length cipher == length plain /\
+	   (nth_in_bounds cipher i == quad32_xor (nth_in_bounds plain i) (aes_encrypt alg key (inc32 icb i) ))))
+=
+  if i = 0 then ()
+  else 
+    match plain with 
+    | [] -> ()
+    | hd :: tl -> 
+      let cipher = gctr_encrypt_recursive icb plain alg key i in  
+      let r_cipher = gctr_encrypt_recursive icb tl alg key (i+1) in     
+      gctr_indexed icb tl alg key (i + 1);
+      assert (nth_in_bounds r_cipher (i-1) == quad32_xor (nth_in_bounds tl (i-1)) (aes_encrypt alg key (inc32 icb (i+1) )));
+      assert( Cons?.tl cipher == r_cipher);
+      //assert (nth_in_bounds r_cipher (i-1) == nth_in_bounds cipher i);
+      
+      assume(False)
+   
   
 (*
 let rec gctr_equivalence (icb:quad32) (plain:gctr_plain) 
@@ -55,4 +146,5 @@ let rec gctr_equivalence (icb:quad32) (plain:gctr_plain)
   match plain with
   | [] -> ()
   | hd :: tl -> gctr_equivalence icb tl alg key (Cons?.tl cipher)
+*)
 *)
